rasimpl: now simplify terms inside substitutions

theories/SubstNotations.v
@@ -95,11 +95,11 @@ Inductive quoted_subst :=
 | qsubst_comp (s t : quoted_subst)
 | qsubst_compr (s : quoted_subst) (r : quoted_ren)
 | qsubst_rcomp (r : quoted_ren) (s : quoted_subst)
-| qsubst_cons (t : cterm) (s : quoted_subst)
+| qsubst_cons (t : quoted_cterm) (s : quoted_subst)
 | qsubst_id
-| qsubst_ren (r : quoted_ren).
+| qsubst_ren (r : quoted_ren)
 
-Inductive quoted_cterm :=
+with quoted_cterm :=
 | qatom (t : cterm)
 | qren (r : quoted_ren) (t : quoted_cterm)
 | qsubst (s : quoted_subst) (t : quoted_cterm).
@@ -126,12 +126,12 @@ Fixpoint unquote_subst q :=
   | qsubst_comp s t => funcomp (subst_cterm (unquote_subst s)) (unquote_subst t)
   | qsubst_compr s r => funcomp (unquote_subst s) (unquote_ren r)
   | qsubst_rcomp r s => funcomp (ren_cterm (unquote_ren r)) (unquote_subst s)
-  | qsubst_cons t s => scons t (unquote_subst s)
+  | qsubst_cons t s => scons (unquote_cterm t) (unquote_subst s)
   | qsubst_id => ids
   | qsubst_ren r => funcomp cvar (unquote_ren r)
-  end.
+  end
 
-Fixpoint unquote_cterm q :=
+with unquote_cterm q :=
   match q with
   | qatom t => t
   | qren r t => ren_cterm (unquote_ren r) (unquote_cterm t)
@@ -265,6 +265,32 @@ Definition test_qren_id r : qren_id_view r :=
   | r => not_qren_id r
   end.
 
+Inductive qsubst_ren_id_view : quoted_subst → Type :=
+| is_qsubst_ren r : qsubst_ren_id_view (qsubst_ren r)
+| is_qsubst_id : qsubst_ren_id_view qsubst_id
+| not_qsubst_ren_id s : qsubst_ren_id_view s.
+
+Definition test_qsubst_ren_id s : qsubst_ren_id_view s :=
+  match s with
+  | qsubst_ren r => is_qsubst_ren r
+  | qsubst_id => is_qsubst_id
+  | s => not_qsubst_ren_id s
+  end.
+
+(* TODO Could be improved like apply_ren *)
+Fixpoint apply_subst (s : quoted_subst) (n : quoted_nat) : quoted_cterm :=
+  match s, n with
+  | qsubst_atom s, _ => qatom (s (unquote_nat n))
+  | qsubst_id, _ => qatom (cvar (unquote_nat n))
+  | _, qnat_atom n => qatom (unquote_subst s n)
+  | qsubst_comp s1 s2, _ => qsubst s1 (apply_subst s2 n)
+  | qsubst_compr s r, _ => apply_subst s (apply_ren r n)
+  | qsubst_rcomp r s, _ => qren r (apply_subst s n)
+  | qsubst_cons t s, q0 => t
+  | qsubst_cons t s, qS n => apply_subst s n
+  | qsubst_ren r, n => qatom (cvar (unquote_nat (apply_ren r n)))
+  end.
+
 Fixpoint eval_subst (s : quoted_subst) : quoted_subst :=
   match s with
   | qsubst_comp u v =>
@@ -276,7 +302,7 @@ Fixpoint eval_subst (s : quoted_subst) : quoted_subst :=
     | es_comp_r u x y => qsubst_comp (qsubst_comp u x) y
     | es_compr_r u x y => qsubst_compr (qsubst_comp u x) y
     | es_rcomp_r u x y => qsubst_comp (qsubst_compr u x) y
-    | es_cons_r u t s => qsubst_cons (subst_cterm (unquote_subst u) t) (qsubst_comp u s)
+    | es_cons_r u t s => qsubst_cons (qsubst u t) (qsubst_comp u s)
     | es_ren_l r s => qsubst_rcomp r s
     | es_ren_r u r => qsubst_compr u r
     | es_other u v => qsubst_comp u v
@@ -288,8 +314,7 @@ Fixpoint eval_subst (s : quoted_subst) : quoted_subst :=
     | esr_id_l r => qsubst_ren r
     | esr_id_r s => s
     | esr_comp_r s x y => qsubst_compr (qsubst_compr s x) y
-    | esr_cons_r s n r =>
-      qsubst_cons (unquote_subst s (unquote_nat n)) (qsubst_compr s r)
+    | esr_cons_r s n r => qsubst_cons (apply_subst s n) (qsubst_compr s r)
     | esr_ren_l s r => qsubst_ren (qren_comp s r)
     | esr_cons_shift t s => s
     | esr_other s r => qsubst_compr s r
@@ -303,12 +328,12 @@ Fixpoint eval_subst (s : quoted_subst) : quoted_subst :=
     | ers_comp_r r x y => qsubst_comp (qsubst_rcomp r x) y
     | ers_compr_r r x y => qsubst_compr (qsubst_rcomp r x) y
     | ers_rcomp_r r x y => qsubst_rcomp (qren_comp r x) y
-    | ers_cons_r r t s =>
-      qsubst_cons (ren_cterm (unquote_ren r) t) (qsubst_rcomp r s)
+    | ers_cons_r r t s => qsubst_cons (qren r t) (qsubst_rcomp r s)
     | ers_ren_r r s => qsubst_ren (qren_comp r s)
     | ers_other r s => qsubst_rcomp r s
     end
   | qsubst_cons t s =>
+    let t := eval_cterm t in
     let s := eval_subst s in
     qsubst_cons t s
   | qsubst_ren r =>
@@ -318,21 +343,9 @@ Fixpoint eval_subst (s : quoted_subst) : quoted_subst :=
     | not_qren_id r => qsubst_ren r
     end
   | _ => s
-  end.
+  end
 
-Inductive qsubst_ren_id_view : quoted_subst → Type :=
-| is_qsubst_ren r : qsubst_ren_id_view (qsubst_ren r)
-| is_qsubst_id : qsubst_ren_id_view qsubst_id
-| not_qsubst_ren_id s : qsubst_ren_id_view s.
-
-Definition test_qsubst_ren_id s : qsubst_ren_id_view s :=
-  match s with
-  | qsubst_ren r => is_qsubst_ren r
-  | qsubst_id => is_qsubst_id
-  | s => not_qsubst_ren_id s
-  end.
-
-Fixpoint eval_cterm (t : quoted_cterm) : quoted_cterm :=
+with eval_cterm (t : quoted_cterm) : quoted_cterm :=
   match t with
   | qren r t =>
     let r := eval_ren r in
@@ -435,164 +448,183 @@ Proof.
       assumption.
 Qed.
 
-Ltac set_eval_subst na :=
-  lazymatch goal with
-  | |- context [ eval_subst ?s ] =>
-    set (na := eval_subst s) in * ;
-    clearbody na
-  end.
-
-Lemma eval_subst_sound :
-  ∀ s,
-    pointwise_relation _ eq (unquote_subst s) (unquote_subst (eval_subst s)).
+Lemma apply_subst_sound :
+  ∀ s n,
+    unquote_cterm (apply_subst s n) = unquote_subst s (unquote_nat n).
 Proof.
   intros s n.
   induction s in n |- *.
   all: try reflexivity.
-  - cbn. set_eval_subst es1. set_eval_subst es2.
-    destruct eval_subst_comp_c.
-    + cbn in *. unfold funcomp. rewrite IHs2.
-      etransitivity.
-      1:{
-        eapply subst_cterm_morphism. 1: eassumption.
-        reflexivity.
-      }
-      asimpl. reflexivity.
-    + cbn in *. unfold funcomp. rewrite IHs2.
-      etransitivity.
-      1:{
-        eapply subst_cterm_morphism. 1: eassumption.
-        reflexivity.
-      }
-      asimpl. reflexivity.
-    + cbn in *. unfold funcomp in *.
-      erewrite subst_cterm_morphism. 2,3: eauto.
-      asimpl. reflexivity.
-    + cbn in *. unfold funcomp in *.
-      erewrite subst_cterm_morphism. 2,3: eauto.
-      asimpl. reflexivity.
-    + cbn in *. unfold funcomp in *.
-      erewrite subst_cterm_morphism. 2,3: eauto.
-      asimpl. reflexivity.
-    + cbn in *. unfold funcomp.
-      erewrite subst_cterm_morphism. 2,3: eauto.
-      asimpl. destruct n. all: reflexivity.
-    + cbn in *. unfold funcomp in *.
-      rewrite IHs2.
-      rewrite rinstInst'_cterm. apply subst_cterm_morphism. 2: reflexivity.
-      intro. rewrite IHs1. unfold funcomp. reflexivity.
-    + cbn in *. unfold funcomp in *.
-      rewrite IHs2. cbn. rewrite IHs1. reflexivity.
-    + cbn in *. unfold funcomp. rewrite IHs2.
-      erewrite subst_cterm_morphism. 2,3: eauto.
-      reflexivity.
-  - cbn. set_eval_subst es.
-    remember (eval_ren _) as er eqn:e.
-    destruct eval_subst_compr_c.
-    + subst. cbn. unfold funcomp. rewrite IHs.
-      cbn. rewrite <- eval_ren_sound. reflexivity.
-    + unfold funcomp. rewrite eval_ren_sound, <- e. cbn.
-      rewrite IHs. reflexivity.
-    + unfold funcomp. rewrite eval_ren_sound, <- e. cbn.
-      rewrite IHs. reflexivity.
-    + unfold funcomp. rewrite eval_ren_sound, <- e. cbn.
-      rewrite IHs. destruct n. all: reflexivity.
-    + subst. cbn. unfold funcomp. rewrite <- eval_ren_sound.
-      rewrite IHs. reflexivity.
-    + unfold funcomp. rewrite eval_ren_sound, <- e. cbn.
-      rewrite IHs. cbn. reflexivity.
-    + subst. cbn. unfold funcomp. rewrite <- eval_ren_sound.
-      rewrite IHs. reflexivity.
-  - cbn. set_eval_subst es.
-    remember (eval_ren _) as er eqn:e.
-    destruct eval_subst_rcomp_c.
-    + unfold funcomp.
-      erewrite ren_cterm_morphism. 3: reflexivity.
-      2:{ intro. rewrite eval_ren_sound, <- e. reflexivity. }
-      cbn. asimpl. auto.
-    + subst. unfold funcomp. rewrite IHs. cbn. rewrite eval_ren_sound.
-      reflexivity.
-    + subst. unfold funcomp. rewrite IHs. cbn. unfold funcomp.
-      rewrite substRen_cterm. apply subst_cterm_morphism. 2: reflexivity.
-      intro. unfold funcomp. apply ren_cterm_morphism. 2: reflexivity.
-      intro. rewrite <- eval_ren_sound. reflexivity.
-    + subst. unfold funcomp. rewrite IHs. cbn. unfold funcomp.
-      apply ren_cterm_morphism. 2: reflexivity.
-      intro. rewrite <- eval_ren_sound. reflexivity.
-    + subst. unfold funcomp. rewrite IHs. cbn. unfold funcomp.
-      rewrite renRen_cterm. apply ren_cterm_morphism. 2: reflexivity.
-      intro. rewrite <- eval_ren_sound. reflexivity.
-    + subst. unfold funcomp. rewrite IHs. cbn.
-      destruct n.
-      * cbn. apply ren_cterm_morphism. 2: reflexivity.
-        intro. rewrite eval_ren_sound. reflexivity.
-      * cbn. unfold funcomp. apply ren_cterm_morphism. 2: reflexivity.
-        intro. rewrite eval_ren_sound. reflexivity.
-    + subst. unfold funcomp. rewrite IHs. cbn. unfold funcomp.
-      rewrite <- eval_ren_sound. reflexivity.
-    + subst. cbn. unfold funcomp. rewrite IHs.
-      apply ren_cterm_morphism. 2: reflexivity.
-      intro. rewrite eval_ren_sound. reflexivity.
-  - cbn. erewrite scons_morphism. 2,3: eauto.
-    reflexivity.
-  - cbn. remember (eval_ren _) as er eqn:e.
-    destruct test_qren_id.
-    + cbn. unfold funcomp. rewrite eval_ren_sound, <- e.
-      reflexivity.
-    + subst. cbn. unfold funcomp. rewrite <- eval_ren_sound.
-      reflexivity.
+  - cbn. destruct n.
+    + reflexivity.
+    + cbn. rewrite IHs2. reflexivity.
+    + cbn. rewrite IHs2. reflexivity.
+  - cbn. destruct n.
+    + reflexivity.
+    + rewrite IHs. rewrite apply_ren_sound. reflexivity.
+    + cbn. rewrite IHs. rewrite apply_ren_sound. reflexivity.
+  - cbn. destruct n.
+    + reflexivity.
+    + cbn. rewrite IHs. reflexivity.
+    + cbn. rewrite IHs. reflexivity.
+  - cbn. destruct n.
+    + reflexivity.
+    + reflexivity.
+    + cbn. rewrite IHs. reflexivity.
+  - cbn. destruct n.
+    + reflexivity.
+    + cbn. rewrite apply_ren_sound. reflexivity.
+    + cbn. rewrite apply_ren_sound. reflexivity.
 Qed.
 
-Lemma eval_cterm_sound :
-  ∀ t,
+Ltac set_eval_subst na :=
+  lazymatch goal with
+  | eval_subst_sound : ∀ s : quoted_subst, _ |- context [ eval_subst ?s ] =>
+    let IH := fresh "IH" in
+    pose proof (eval_subst_sound s) as IH ;
+    set (na := eval_subst s) in * ;
+    clearbody na
+  end.
+
+Fixpoint eval_subst_sound s :
+    pointwise_relation _ eq (unquote_subst s) (unquote_subst (eval_subst s))
+
+with eval_cterm_sound t :
     unquote_cterm t = unquote_cterm (eval_cterm t).
 Proof.
-  intros t.
-  induction t.
-  - reflexivity.
-  - cbn. remember (eval_cterm _) as et eqn:e in *.
-    destruct et.
-    + remember (eval_ren _) as rr eqn:er.
+  {
+    intros n.
+    destruct s.
+    all: try reflexivity.
+    - cbn. set_eval_subst es1. set_eval_subst es2.
+      destruct eval_subst_comp_c.
+      + cbn in *. unfold funcomp. rewrite IH, IH0.
+        asimpl. reflexivity.
+      + cbn in *. unfold funcomp. rewrite IH, IH0.
+        asimpl. reflexivity.
+      + cbn in *. unfold funcomp in *.
+        erewrite subst_cterm_morphism. 2,3: eauto.
+        asimpl. reflexivity.
+      + cbn in *. unfold funcomp in *.
+        erewrite subst_cterm_morphism. 2,3: eauto.
+        asimpl. reflexivity.
+      + cbn in *. unfold funcomp in *.
+        erewrite subst_cterm_morphism. 2,3: eauto.
+        asimpl. reflexivity.
+      + cbn in *. unfold funcomp.
+        erewrite subst_cterm_morphism. 2,3: eauto.
+        asimpl. destruct n. all: reflexivity.
+      + cbn in *. unfold funcomp in *.
+        rewrite IH, IH0.
+        rewrite rinstInst'_cterm. reflexivity.
+      + cbn in *. unfold funcomp in *.
+        rewrite IH, IH0. reflexivity.
+      + cbn in *. unfold funcomp. rewrite IH, IH0. reflexivity.
+    - cbn. set_eval_subst es.
+      remember (eval_ren _) as er eqn:e.
+      destruct eval_subst_compr_c.
+      + subst. cbn. unfold funcomp. rewrite IH.
+        cbn. rewrite <- eval_ren_sound. reflexivity.
+      + unfold funcomp. rewrite eval_ren_sound, <- e. cbn.
+        rewrite IH. reflexivity.
+      + unfold funcomp. rewrite eval_ren_sound, <- e. cbn.
+        rewrite IH. reflexivity.
+      + unfold funcomp. rewrite eval_ren_sound, <- e. cbn.
+        rewrite IH. destruct n. 2: reflexivity.
+        cbn. rewrite apply_subst_sound. reflexivity.
+      + subst. cbn. unfold funcomp. rewrite <- eval_ren_sound.
+        rewrite IH. reflexivity.
+      + unfold funcomp. rewrite eval_ren_sound, <- e. cbn.
+        rewrite IH. cbn. reflexivity.
+      + subst. cbn. unfold funcomp. rewrite <- eval_ren_sound.
+        rewrite IH. reflexivity.
+    - cbn. set_eval_subst es.
+      remember (eval_ren _) as er eqn:e.
+      destruct eval_subst_rcomp_c.
+      + unfold funcomp.
+        erewrite ren_cterm_morphism. 3: reflexivity.
+        2:{ intro. rewrite eval_ren_sound, <- e. reflexivity. }
+        cbn. asimpl. auto.
+      + subst. unfold funcomp. rewrite IH. cbn. rewrite eval_ren_sound.
+        reflexivity.
+      + subst. unfold funcomp. rewrite IH. cbn. unfold funcomp.
+        rewrite substRen_cterm. apply subst_cterm_morphism. 2: reflexivity.
+        intro. unfold funcomp. apply ren_cterm_morphism. 2: reflexivity.
+        intro. rewrite <- eval_ren_sound. reflexivity.
+      + subst. unfold funcomp. rewrite IH. cbn. unfold funcomp.
+        apply ren_cterm_morphism. 2: reflexivity.
+        intro. rewrite <- eval_ren_sound. reflexivity.
+      + subst. unfold funcomp. rewrite IH. cbn. unfold funcomp.
+        rewrite renRen_cterm. apply ren_cterm_morphism. 2: reflexivity.
+        intro. rewrite <- eval_ren_sound. reflexivity.
+      + subst. unfold funcomp. rewrite IH. cbn.
+        destruct n.
+        * cbn. apply ren_cterm_morphism. 2: reflexivity.
+          intro. rewrite eval_ren_sound. reflexivity.
+        * cbn. unfold funcomp. apply ren_cterm_morphism. 2: reflexivity.
+          intro. rewrite eval_ren_sound. reflexivity.
+      + subst. unfold funcomp. rewrite IH. cbn. unfold funcomp.
+        rewrite <- eval_ren_sound. reflexivity.
+      + subst. cbn. unfold funcomp. rewrite IH.
+        apply ren_cterm_morphism. 2: reflexivity.
+        intro. rewrite eval_ren_sound. reflexivity.
+    - cbn. erewrite scons_morphism. 2,3: eauto.
+      reflexivity.
+    - cbn. remember (eval_ren _) as er eqn:e.
       destruct test_qren_id.
-      * cbn. erewrite ren_cterm_morphism. 3: reflexivity.
-        2:{ intro. rewrite eval_ren_sound, <- er. reflexivity. }
-        cbn. asimpl. assumption.
-      * subst. cbn. rewrite IHt. cbn.
-        eapply ren_cterm_morphism. 2: reflexivity.
-        intro. apply eval_ren_sound.
-    + cbn. rewrite IHt. cbn. rewrite renRen_cterm.
-      apply ren_cterm_morphism. 2: reflexivity.
-      intro. unfold funcomp. rewrite <- eval_ren_sound. reflexivity.
-    + cbn. rewrite IHt. cbn.
-      rewrite substRen_cterm.
-      apply subst_cterm_morphism. 2: reflexivity.
-      intro. unfold funcomp.
-      rewrite rinstInst'_cterm.
-      apply subst_cterm_morphism. 2: reflexivity.
-      intro. unfold funcomp.
-      rewrite <- eval_ren_sound. reflexivity.
-  - cbn. remember (eval_cterm _) as et eqn:e in *.
-    destruct et.
-    + remember (eval_subst _) as ss eqn:es in *.
-      rewrite IHt. cbn.
-      destruct test_qsubst_ren_id.
-      * cbn. erewrite subst_cterm_morphism. 3: reflexivity.
-        2:{ intro. rewrite eval_subst_sound, <- es. reflexivity. }
-        cbn. rewrite rinstInst'_cterm. reflexivity.
-      * cbn. erewrite subst_cterm_morphism. 3: reflexivity.
-        2:{ intro. rewrite eval_subst_sound, <- es. reflexivity. }
-        cbn. asimpl. reflexivity.
-      * subst. cbn.
+      + cbn. unfold funcomp. rewrite eval_ren_sound, <- e.
+        reflexivity.
+      + subst. cbn. unfold funcomp. rewrite <- eval_ren_sound.
+        reflexivity.
+  }
+  {
+    destruct t.
+    - reflexivity.
+    - cbn. remember (eval_cterm _) as et eqn:e in *.
+      destruct et.
+      + remember (eval_ren _) as rr eqn:er.
+        destruct test_qren_id.
+        * rewrite eval_cterm_sound, <- e.
+          cbn. erewrite ren_cterm_morphism. 3: reflexivity.
+          2:{ intro. rewrite eval_ren_sound, <- er. reflexivity. }
+          cbn. asimpl. reflexivity.
+        * subst. cbn. rewrite eval_cterm_sound, <- e. cbn.
+          eapply ren_cterm_morphism. 2: reflexivity.
+          intro. apply eval_ren_sound.
+      + cbn. rewrite eval_cterm_sound, <- e. cbn. rewrite renRen_cterm.
+        apply ren_cterm_morphism. 2: reflexivity.
+        intro. unfold funcomp. rewrite <- eval_ren_sound. reflexivity.
+      + cbn. rewrite eval_cterm_sound, <- e. cbn.
+        rewrite substRen_cterm.
+        apply subst_cterm_morphism. 2: reflexivity.
+        intro. unfold funcomp.
+        rewrite rinstInst'_cterm.
+        apply subst_cterm_morphism. 2: reflexivity.
+        intro. unfold funcomp.
+        rewrite <- eval_ren_sound. reflexivity.
+    - cbn. remember (eval_cterm _) as et eqn:e in *.
+      destruct et.
+      + remember (eval_subst _) as ss eqn:es in *.
+        rewrite eval_cterm_sound, <- e. cbn.
+        destruct test_qsubst_ren_id.
+        * cbn. erewrite subst_cterm_morphism. 3: reflexivity.
+          2:{ intro. rewrite eval_subst_sound, <- es. reflexivity. }
+          cbn. rewrite rinstInst'_cterm. reflexivity.
+        * cbn. erewrite subst_cterm_morphism. 3: reflexivity.
+          2:{ intro. rewrite eval_subst_sound, <- es. reflexivity. }
+          cbn. asimpl. reflexivity.
+        * subst. cbn.
+          eapply subst_cterm_morphism. 2: reflexivity.
+          intro. apply eval_subst_sound.
+      + cbn. rewrite eval_cterm_sound, <- e. cbn. rewrite renSubst_cterm.
+        apply subst_cterm_morphism. 2: reflexivity.
+        intro. unfold funcomp. rewrite <- eval_subst_sound. reflexivity.
+      + cbn. rewrite eval_cterm_sound, <- e. cbn. rewrite substSubst_cterm.
         eapply subst_cterm_morphism. 2: reflexivity.
-        intro. apply eval_subst_sound.
-    + cbn. rewrite IHt. cbn. rewrite renSubst_cterm.
-      apply subst_cterm_morphism. 2: reflexivity.
-      intro. unfold funcomp. rewrite <- eval_subst_sound. reflexivity.
-    + cbn. rewrite IHt. cbn. rewrite substSubst_cterm.
-      eapply subst_cterm_morphism. 2: reflexivity.
-      intro. unfold funcomp.
-      eapply subst_cterm_morphism. 2: reflexivity.
-      intro. rewrite <- eval_subst_sound. reflexivity.
+        intro. unfold funcomp.
+        eapply subst_cterm_morphism. 2: reflexivity.
+        intro. rewrite <- eval_subst_sound. reflexivity.
+  }
 Qed.
 
 (** Quoting **)
@@ -657,14 +689,15 @@ Ltac quote_subst s :=
     let qr := quote_ren r in
     constr:(qsubst_compr qs qr)
   | scons ?t ?s =>
+    let qt := quote_cterm t in
     let q := quote_subst s in
-    constr:(qsubst_cons t q)
+    constr:(qsubst_cons qt q)
   | ids => constr:(qsubst_id)
   | cvar => constr:(qsubst_id)
   | _ => constr:(qsubst_atom s)
-  end.
+  end
 
-Ltac quote_cterm t :=
+with quote_cterm t :=
   lazymatch t with
   | ren_cterm ?r ?t =>
     let qr := quote_ren r in
@@ -721,7 +754,7 @@ Ltac post_process :=
     unquote_cterm eval_cterm test_qren_id test_qsubst_ren_id
     unquote_ren eval_ren apply_ren eval_ren_comp_c
     unquote_subst eval_subst eval_subst_compr_c eval_subst_comp_c
-    eval_subst_rcomp_c
+    eval_subst_rcomp_c apply_subst
     unquote_nat
     ren_cterm subst_cterm scons
   ] ;
@@ -732,7 +765,7 @@ Ltac post_process_in h :=
     unquote_cterm eval_cterm test_qren_id test_qsubst_ren_id
     unquote_ren eval_ren apply_ren eval_ren_comp_c
     unquote_subst eval_subst eval_subst_compr_c eval_subst_comp_c
-    eval_subst_rcomp_c
+    eval_subst_rcomp_c apply_subst
     unquote_nat
     ren_cterm subst_cterm scons
   ] in h ;
@@ -753,7 +786,7 @@ Hint Mode CTermSimplification + - : typeclass_instances.
       unquote_cterm eval_cterm test_qren_id test_qsubst_ren_id
       unquote_ren eval_ren apply_ren eval_ren_comp_c
       unquote_subst eval_subst eval_subst_compr_c eval_subst_comp_c
-      eval_subst_rcomp_c
+      eval_subst_rcomp_c apply_subst
       unquote_nat
       ren_cterm subst_cterm scons
     ]
@@ -780,7 +813,7 @@ Hint Mode RenSimplification + - : typeclass_instances.
       unquote_cterm eval_cterm test_qren_id test_qsubst_ren_id
       unquote_ren eval_ren apply_ren eval_ren_comp_c
       unquote_subst eval_subst eval_subst_compr_c eval_subst_comp_c
-      eval_subst_rcomp_c
+      eval_subst_rcomp_c apply_subst
       unquote_nat
       ren_cterm subst_cterm scons
     ]
@@ -807,7 +840,7 @@ Hint Mode CSubstSimplification + - : typeclass_instances.
       unquote_cterm eval_cterm test_qren_id test_qsubst_ren_id
       unquote_ren eval_ren apply_ren eval_ren_comp_c
       unquote_subst eval_subst eval_subst_compr_c eval_subst_comp_c
-      eval_subst_rcomp_c
+      eval_subst_rcomp_c apply_subst
       unquote_nat
       ren_cterm subst_cterm scons
     ]
